examples/lambda/completeness/boehm_treeScript.sml
@@ -1,0 +1,186 @@
+(*---------------------------------------------------------------------------*
+ * boehm_treeScript.sml: (Effective) Boehm Trees (Chapter 10 of [1])         *
+ *---------------------------------------------------------------------------*)
+
+open HolKernel boolLib Parse bossLib;
+
+(* core theories *)
+open optionTheory arithmeticTheory pred_setTheory listTheory llistTheory
+     ltreeTheory pathTheory posetTheory hurdUtils;
+
+open binderLib termTheory appFOLDLTheory chap2Theory chap3Theory
+     head_reductionTheory standardisationTheory solvableTheory pure_dBTheory;
+
+val _ = new_theory "boehm_tree";
+
+val o_DEF = combinTheory.o_DEF; (* cannot directly open combinTheory *)
+
+(* A dB-term M is hnf if its corresponding Lambda term is hnf *)
+Overload dhnf = “hnf o toTerm”
+
+Theorem dhnf_fromTerm[simp] :
+    !M. dhnf (fromTerm M) <=> hnf M
+Proof
+    rw [o_DEF]
+QED
+
+(* Translations from LAMl to dABSi.
+
+   Some samples for guessing out the statements of this theorem:
+
+> SIMP_CONV arith_ss [dLAM_def, lift_def, sub_def, lift_sub]
+                     “dLAM v1 (dLAM v0 t)”;
+# val it =
+   |- dLAM v1 (dLAM v0 t) =
+      dABS (dABS ([dV 1/v1 + 2] ([dV 0/v0 + 2] (lift (lift t 0) 1)))): thm
+
+> SIMP_CONV arith_ss [dLAM_def, lift_def, sub_def, lift_sub]
+                     “dLAM v2 (dLAM v1 (dLAM v0 t))”;
+# val it =
+   |- dLAM v2 (dLAM v1 (dLAM v0 t)) =
+      dABS
+        (dABS
+           (dABS ([dV 2/v2 + 3]
+                    ([dV 1/v1 + 3]
+                       ([dV 0/v0 + 3]
+                          (lift (lift (lift t 0) 1) 2)))))): thm
+ *)
+Theorem LAMl_to_dABSi :
+    !vs. ALL_DISTINCT (vs :num list) ==>
+         let n = LENGTH vs;
+             body = FOLDL lift t (GENLIST I n);
+             phi = ZIP (GENLIST dV n, MAP (\i. i + n) (REVERSE vs))
+         in LAMl vs t = dABSi n (body ISUB phi)
+Proof
+    Induct_on ‘vs’ >- rw [isub_def]
+ >> rw [isub_def, GSYM SNOC_APPEND, MAP_SNOC, FUNPOW_SUC, GENLIST, FOLDL_SNOC,
+        dLAM_def]
+ >> fs []
+ >> qabbrev_tac ‘n = LENGTH vs’
+ >> rw [lift_dABSi]
+ >> Q.PAT_X_ASSUM ‘LAMl vs t = _’ K_TAC
+ >> qabbrev_tac ‘N = FOLDL lift t (GENLIST I n)’
+ >> qabbrev_tac ‘Ms = GENLIST dV n’
+ >> qabbrev_tac ‘Vs = MAP (\i. i + n) (REVERSE vs)’
+ >> Know ‘lift (N ISUB ZIP (Ms,Vs)) n =
+          (lift N n) ISUB (ZIP (MAP (\e. lift e n) Ms,MAP SUC Vs))’
+ >- (MATCH_MP_TAC lift_isub \\
+     rw [Abbr ‘Ms’, Abbr ‘Vs’, EVERY_MEM, MEM_MAP] >> rw [])
+ >> Rewr'
+ >> ‘MAP SUC Vs = MAP (\i. i + SUC n) (REVERSE vs)’
+       by (rw [LIST_EQ_REWRITE, EL_MAP, Abbr ‘Vs’]) >> POP_ORW
+ >> qunabbrev_tac ‘Vs’ (* now useless *)
+ >> rw [sub_def, GSYM ADD1]
+ >> ‘MAP (\e. lift e n) Ms = Ms’
+       by (rw [LIST_EQ_REWRITE, EL_MAP, Abbr ‘Ms’]) >> POP_ORW
+ >> qabbrev_tac ‘Ns = MAP (\i. i + SUC n) (REVERSE vs)’
+ >> qabbrev_tac ‘N' = lift N n’
+ >> Suff ‘N' ISUB ZIP (SNOC (dV n) Ms,SNOC (h + SUC n) Ns) =
+          [dV n/h + SUC n] (N' ISUB ZIP (Ms,Ns))’ >- rw []
+ >> MATCH_MP_TAC isub_SNOC
+ >> rw [Abbr ‘Ms’, Abbr ‘Ns’, MEM_EL, EL_MAP]
+ >> rename1 ‘~(i < n)’
+ >> ‘LENGTH (REVERSE vs) = n’ by rw [Abbr ‘n’]
+ >> CCONTR_TAC >> gs [EL_MAP]
+ >> ‘h = EL i (REVERSE vs)’ by rw []
+ >> Suff ‘MEM h (REVERSE vs)’ >- rw [MEM_REVERSE]
+ >> Q.PAT_X_ASSUM ‘~MEM h vs’ K_TAC
+ >> ‘LENGTH (REVERSE vs) = n’ by rw [Abbr ‘n’]
+ >> REWRITE_TAC [MEM_EL]
+ >> Q.EXISTS_TAC ‘i’ >> art []
+QED
+
+(* |- !t vs.
+        ALL_DISTINCT vs ==>
+        LAMl vs t =
+        dABSi (LENGTH vs)
+          (FOLDL lift t (GENLIST I (LENGTH vs)) ISUB
+           ZIP (GENLIST dV (LENGTH vs),MAP (\i. i + LENGTH vs) (REVERSE vs)))
+ *)
+Theorem LAMl_to_dABSi_applied[local] =
+    GEN_ALL (SIMP_RULE std_ss [LET_DEF] LAMl_to_dABSi)
+
+(* dB version of hnf_cases (only the ==> direction) *)
+Theorem dhnf_cases :
+    !M. dhnf M ==> ?n y Ms. M = dABSi n (dV y @* Ms)
+Proof
+    RW_TAC std_ss [hnf_cases]
+ >> qabbrev_tac ‘n = LENGTH vs’
+ >> Q.EXISTS_TAC ‘n’
+ >> Know ‘fromTerm (toTerm M) = fromTerm (LAMl vs (VAR y @* args))’
+ >- (art [fromTerm_11])
+ >> Q.PAT_X_ASSUM ‘toTerm M = LAMl vs (VAR y @* args)’ K_TAC
+ >> rw [fromTerm_LAMl, fromTerm_appstar]
+ >> qabbrev_tac ‘vs' = MAP s2n vs’
+ >> qabbrev_tac ‘Ms = MAP fromTerm args’
+ >> qabbrev_tac ‘y' = s2n y’
+ >> Know ‘LAMl vs' (dV y' @* Ms) =
+          dABSi (LENGTH vs')
+            (FOLDL lift (dV y' @* Ms) (GENLIST I (LENGTH vs')) ISUB
+             ZIP (GENLIST dV (LENGTH vs'),
+                  MAP (\i. i + LENGTH vs') (REVERSE vs')))’
+ >- (MATCH_MP_TAC LAMl_to_dABSi_applied \\
+     qunabbrev_tac ‘vs'’ \\
+     MATCH_MP_TAC ALL_DISTINCT_MAP_INJ >> rw [])
+ >> ‘LENGTH vs' = n’ by rw [Abbr ‘vs'’] >> POP_ORW
+ >> Rewr'
+ >> simp [FOLDL_lift_appstar, isub_appstar]
+ >> Know ‘FOLDL lift (dV y') (GENLIST I n) = dV (y' + n)’
+ >- (KILL_TAC \\
+     Induct_on ‘n’ >> rw [GENLIST, FOLDL_SNOC])
+ >> Rewr'
+ >> qabbrev_tac ‘Ms' = MAP (\e. FOLDL lift e (GENLIST I n)) Ms’
+ >> reverse (Cases_on ‘MEM y vs’)
+ >- (‘~MEM y' vs'’ by (rw [Abbr ‘y'’, Abbr ‘vs'’, MEM_MAP]) \\
+     ‘~MEM y' (REVERSE vs')’ by PROVE_TAC [MEM_REVERSE] \\
+     Suff ‘dV (y' + n) ISUB ZIP (GENLIST dV n,MAP (\i. i + n) (REVERSE vs')) =
+           dV (y' + n)’ >- (Rewr' >> METIS_TAC []) \\
+     MATCH_MP_TAC isub_dV_fresh \\
+     qabbrev_tac ‘l1 = GENLIST dV n’ \\
+     qabbrev_tac ‘l2 = MAP (\i. i + n) (REVERSE vs')’ \\
+    ‘LENGTH l1 = n’ by rw [Abbr ‘l1’] \\
+    ‘LENGTH l2 = n’ by rw [Abbr ‘l2’, Abbr ‘n’, Abbr ‘vs'’] \\
+     simp [DOM_ALT_MAP_SND, MAP_ZIP] \\
+     rw [Abbr ‘l2’, MEM_MAP])
+ (* stage work *)
+ >> ‘MEM y' vs'’ by (rw [Abbr ‘y'’, Abbr ‘vs'’, MEM_MAP])
+ >> ‘MEM y' (REVERSE vs')’ by PROVE_TAC [MEM_REVERSE]
+ >> ‘?j. j < LENGTH (REVERSE vs') /\ y' = EL j (REVERSE vs')’
+        by METIS_TAC [MEM_EL]
+ >> ‘LENGTH (REVERSE vs') = n’ by rw [Abbr ‘vs'’, Abbr ‘n’]
+ >> qabbrev_tac ‘Ns = MAP (\i. i + n) (REVERSE vs')’
+ >> ‘LENGTH Ns = n’ by rw [Abbr ‘Ns’]
+ >> Know ‘ALL_DISTINCT Ns’
+ >- (qunabbrev_tac ‘Ns’ \\
+     MATCH_MP_TAC ALL_DISTINCT_MAP_INJ >> rw [] \\
+     qunabbrev_tac ‘vs'’ \\
+     MATCH_MP_TAC ALL_DISTINCT_MAP_INJ >> rw [])
+ >> DISCH_TAC
+ >> Suff ‘dV (y' + n) ISUB ZIP (GENLIST dV n,Ns) = EL j (GENLIST dV n)’
+ >- (Rewr' \\
+     simp [EL_GENLIST] >> METIS_TAC [])
+ >> MATCH_MP_TAC isub_dV_once >> simp []
+ >> CONJ_TAC >- (rw [Abbr ‘Ns’, EL_MAP])
+ >> Q.X_GEN_TAC ‘i’ >> DISCH_TAC
+ >> ‘n <= EL i Ns’ by rw [Abbr ‘Ns’, EL_MAP]
+ >> Suff ‘FVS (ZIP (GENLIST dV n,Ns)) = count n’ >- rw []
+ >> Q.PAT_X_ASSUM ‘LENGTH Ns = n’ MP_TAC
+ >> KILL_TAC >> Q.ID_SPEC_TAC ‘Ns’
+ >> Induct_on ‘n’ >> rw [dFVS_def]
+ >> ‘Ns <> []’ by rw [NOT_NIL_EQ_LENGTH_NOT_0]
+ >> ‘LENGTH (FRONT Ns) = n’ by rw [LENGTH_FRONT]
+ >> ‘Ns = SNOC (LAST Ns) (FRONT Ns)’
+      by (rw [APPEND_FRONT_LAST, SNOC_APPEND]) >> POP_ORW
+ >> Q.PAT_X_ASSUM ‘!Ns. LENGTH Ns = n ==> P’ (MP_TAC o (Q.SPEC ‘FRONT Ns’))
+ >> rw [GENLIST, COUNT_SUC, dFVS_SNOC, ZIP_SNOC, dFV_def]
+ >> SET_TAC []
+QED
+
+val _ = export_theory ();
+val _ = html_theory "boehm_tree";
+
+(* References:
+
+   [1] Barendregt, H.P.: The lambda calculus, its syntax and semantics.
+       College Publications, London (1984).
+ *)
